Semantics/TreeToGraph.thy
@@ -240,33 +240,6 @@ lemmas RepE\<^marker>\<open>tag invisible\<close> =
   ZeroExtendNodeE
   LeafNodeE
 
-(* ======== TODO: Functions for re-calculating stamps ========== *)
-fun stamp_unary :: "IRUnaryOp \<Rightarrow> Stamp \<Rightarrow> Stamp" where
-  "stamp_unary op (IntegerStamp b lo hi) = unrestricted_stamp (IntegerStamp b lo hi)" |
-  (* for now... *)
-  "stamp_unary op _ = IllegalStamp"
-
-definition fixed_32 :: "IRBinaryOp set" where
-  "fixed_32 = {BinIntegerEquals, BinIntegerLessThan, BinIntegerBelow}"
-
-fun stamp_binary :: "IRBinaryOp \<Rightarrow> Stamp \<Rightarrow> Stamp \<Rightarrow> Stamp" where
-  "stamp_binary op (IntegerStamp b1 lo1 hi1) (IntegerStamp b2 lo2 hi2) =
-    (case op \<in> fixed_32 of True \<Rightarrow> unrestricted_stamp (IntegerStamp 32 lo1 hi1) |
-    False \<Rightarrow>
-    (if (b1 = b2) then unrestricted_stamp (IntegerStamp b1 lo1 hi1) else IllegalStamp))" |
-  (* for now... *)
-  "stamp_binary op _ _ = IllegalStamp"
-
-fun stamp_expr :: "IRExpr \<Rightarrow> Stamp" where
-  "stamp_expr (UnaryExpr op x) = stamp_unary op (stamp_expr x)" |
-  "stamp_expr (BinaryExpr bop x y) = stamp_binary bop (stamp_expr x) (stamp_expr y)" |
-  "stamp_expr (ConstantExpr val) = constantAsStamp val" |
-  "stamp_expr (LeafExpr i s) = s" |
-  "stamp_expr (ParameterExpr i s) = s" |
-  "stamp_expr (ConditionalExpr c t f) = meet (stamp_expr t) (stamp_expr f)"
-
-export_code stamp_unary stamp_binary stamp_expr
-
 fun unary_node :: "IRUnaryOp \<Rightarrow> ID \<Rightarrow> IRNode" where
   "unary_node UnaryAbs v = AbsNode v" |
   "unary_node UnaryNot v = NotNode v" |
